examples/dexter/Dexter.v
@@ -1,0 +1,115 @@
+(* A token-asset exchange contract based on Dexter
+   https://gitlab.com/camlcase-dev/dexter/-/blob/f4ef07ea672a1397b58c2134b3437bb5ef69bcaa/dexter-contracts-ligo/dexter.ligo *)
+From Coq Require Import ZArith_base.
+From Coq Require Import List. Import ListNotations.
+From ConCert.Utils Require Import RecordUpdate.
+From ConCert.Execution Require Import Blockchain.
+From ConCert.Execution Require Import ContractCommon.
+From ConCert.Execution Require Import Monads.
+From ConCert.Execution Require Import Serializable.
+From ConCert.Examples.EIP20 Require EIP20Token.
+
+(* A liquidity exchange contract inspired by the Dexter contract.
+   Allows for exchanging tokens to money, and allows the owner to add tokens to the
+   reserve held by this contract. *)
+Section Dexter.
+  Context {BaseTypes : ChainBase}.
+  Set Primitive Projections.
+  Set Nonrecursive Elimination Schemes.
+  Open Scope N_scope.
+
+  Record exchange_param :=
+    build_exchange_param {
+      exchange_owner : Address;
+      tokens_sold : N;
+    }.
+
+  Inductive Msg :=
+    | tokens_to_asset : exchange_param -> Msg
+    | add_to_tokens_reserve : Msg.
+
+  Record Setup :=
+    build_setup {
+      token_caddr_ : Address;
+      token_pool_ : N;
+    }.
+
+  Record State :=
+    build_state {
+      token_pool : N;
+      price_history : list Amount;
+      token_caddr : Address;
+    }.
+
+  MetaCoq Run (make_setters State).
+  MetaCoq Run (make_setters Setup).
+
+  Section Serialization.
+
+  Global Instance exchange_paramserializable : Serializable exchange_param :=
+    Derive Serializable exchange_param_rect <build_exchange_param>.
+
+  Global Instance DexterMsg_serializable : Serializable Msg :=
+    Derive Serializable Msg_rect <tokens_to_asset, add_to_tokens_reserve>.
+
+  Global Instance setup_serializable : Serializable Setup :=
+    Derive Serializable Setup_rect <build_setup>.
+
+  Global Instance state_serializable : Serializable State :=
+    Derive Serializable State_rect <build_state>.
+
+  End Serialization.
+
+  (* calculates exchange rate *)
+  Open Scope Z_scope.
+  Definition getInputPrice (tokens_to_be_sold : Amount)
+                          (tokens_reserve : Amount)
+                          (asset_reserve : Amount) :=
+    Z.div (tokens_to_be_sold * 997 * asset_reserve) (tokens_reserve * 1000 + tokens_to_be_sold * 997).
+
+  Definition begin_exchange_tokens_to_assets (dexter_asset_reserve : Amount)
+                                            (caller : Address)
+                                            (params : exchange_param)
+                                            (dexter_caddr : Address)
+                                            (state : State)
+                                            : option (State * (list ActionBody)) :=
+    do _ <- throwIf (negb (address_eqb caller params.(exchange_owner))) ;
+    let tokens_to_sell := Z.of_N params.(tokens_sold) in
+    let tokens_price := getInputPrice tokens_to_sell (Z.of_N state.(token_pool)) dexter_asset_reserve in
+    (* send out asset transfer to transfer owner, and send a token transfer message to the FA2 token *)
+    let asset_transfer_msg := act_transfer params.(exchange_owner) tokens_price in
+    let token_transfer_param := 
+      EIP20Token.transfer_from params.(exchange_owner) dexter_caddr params.(tokens_sold)  in
+    let token_transfer_msg := act_call state.(token_caddr) 0%Z (@serialize EIP20Token.Msg _ (token_transfer_param)) in
+    let new_state := state<|token_pool := N.add state.(token_pool) params.(tokens_sold)|>
+                          <| price_history := state.(price_history) ++ [tokens_price]|> in
+    Some (new_state, [asset_transfer_msg; token_transfer_msg]).
+
+  Open Scope Z_scope.
+  Definition receive (chain : Chain)
+                     (ctx : ContractCallContext)
+                     (state : State)
+                     (maybe_msg : option Msg)
+                     : option (State * list ActionBody) :=
+    let sender := ctx.(ctx_from) in
+    let caddr := ctx.(ctx_contract_address) in
+    let dexter_balance := ctx.(ctx_contract_balance) in
+    match maybe_msg with
+    | Some (tokens_to_asset params) => begin_exchange_tokens_to_assets dexter_balance sender params caddr state
+    (* Ignore any other type of call to this contract *)
+    | _ => Some (state, [])
+    end.
+
+  Definition init (chain : Chain)
+                  (ctx : ContractCallContext)
+                  (setup : Setup) : option State :=
+    Some {|
+      token_pool := setup.(token_pool_);
+      token_caddr := setup.(token_caddr_);
+      price_history := []
+    |}.
+
+  Definition contract : Contract Setup Msg State :=
+    build_contract init receive.
+
+End Dexter.
