examples/dexter/DexterPrinters.v
@@ -1,0 +1,49 @@
+From ConCert.Execution Require Import Blockchain.
+From ConCert.Execution Require Import Serializable.
+From ConCert.Execution.Test Require Import QCTest.
+From ConCert.Examples.Dexter Require Import Dexter.
+From ConCert.Examples.EIP20 Require Import EIP20Token.
+From ConCert.Examples.EIP20 Require Import EIP20TokenPrinters.
+
+Local Open Scope string_scope.
+
+Instance showDexterExchangeParam : Show Dexter.exchange_param :=
+{|
+  show t := "exchange{"
+            ++ "exchange_owner: " ++ show t.(exchange_owner) ++ sep
+            ++ "tokens_sold: " ++ show t.(tokens_sold)
+            ++ "}"
+|}.
+
+Instance showDexterMsg : Show Dexter.Msg :=
+{|
+  show m := match m with
+            | tokens_to_asset param => "token_to_asset " ++ show param
+            | add_to_tokens_reserve => "add_to_tokens_reserve"
+            end
+|}.
+
+Instance showDexterState : Show Dexter.State :=
+{|
+  show t := "DexterState{"
+            ++ "token_caddr: " ++ show t.(token_caddr) ++ sep
+            ++ "token_pool: " ++ show t.(token_pool) ++ sep
+            ++ "price_history: " ++ show t.(price_history)
+            ++ "}"
+|}.
+
+Instance showDexterSetup : Show Dexter.Setup :=
+{|
+  show t := "DexterSetup{"
+            ++ "token_caddr_: " ++ show t.(token_caddr_) ++ sep
+            ++ "token_pool_: " ++ show t.(token_pool_)
+            ++ "}"
+|}.
+
+Instance showSerializedMsg : Show SerializedValue :=
+  Derive Show Msg <
+    Dexter.Msg,
+    Dexter.Setup,
+    EIP20Token.Msg,
+    EIP20Token.Setup
+  >.
