examples/dexter/DexterTests.v
@@ -1,0 +1,199 @@
+
+From ConCert.Utils Require Import Extras.
+From ConCert.Execution Require Import Blockchain.
+From ConCert.Execution Require Import Serializable.
+From ConCert.Execution Require Import Containers.
+From ConCert.Execution Require Import ResultMonad.
+From ConCert.Execution Require Import Monads.
+From ConCert.Execution.Test Require Import QCTest.
+From ConCert.Examples.Dexter Require Import Dexter.
+From ConCert.Examples.Dexter Require Import DexterPrinters.
+From ConCert.Examples.Dexter Require Import DexterGens.
+From ConCert.Examples.EIP20 Require Import EIP20Token.
+From Coq Require Import ZArith_base.
+From Coq Require Import List. Import ListNotations.
+
+
+Definition token_pool_size : N := 100.
+
+Definition token_setup : EIP20Token.Setup := {|
+  EIP20Token.owner := creator;
+  EIP20Token.init_amount := token_pool_size;
+|}.
+
+Definition token_caddr : Address := addr_of_Z 128.
+Definition dexter_caddr : Address := addr_of_Z 129.
+
+(* Dexter will have 60 tokens in reverse initially *)
+Definition dexter_setup : Dexter.Setup := {|
+  token_caddr_ := token_caddr;
+  token_pool_  := (token_pool_size - 40);  
+|}.
+
+Definition add_as_operator_act owner operator tokens :=
+  build_call owner token_caddr 0 (EIP20Token.approve operator tokens). 
+
+Definition exchange_tokens_to_money_act owner amount :=
+  build_call owner dexter_caddr 0 (Dexter.tokens_to_asset {|
+    exchange_owner := owner;
+    tokens_sold := amount;
+  |}).
+
+(* Setup a chain with token contract, and dexter contract deployed.
+   Also adds some tokens to person_1 and dexter contract, and adds some operators on the fa2 contract *)
+Definition chain : ChainBuilder :=
+  unpack_result (TraceGens.add_block builder_initial
+  [  (* Give 10 to person 1 *)
+    build_transfer creator person_1 10 ;
+    (* Deploy contracts *)
+    build_deploy creator 0 EIP20Token.contract token_setup ;
+    build_deploy creator 30 Dexter.contract dexter_setup ;
+    (* Tranfer tokens to exchange contract and person1 *)
+    build_call creator token_caddr 0 (EIP20Token.transfer person_1 40%N) ;
+    build_call creator token_caddr 0 (EIP20Token.transfer dexter_caddr (token_pool_size - 40)%N) ;
+    (* Let dexter transfer tokens on behalf of person_1 and person_2 *)
+    add_as_operator_act person_1 dexter_caddr token_pool_size ;
+    add_as_operator_act person_2 dexter_caddr token_pool_size
+  ]).
+
+Definition add_block_with_acts (c : ChainBuilder) acts :=
+  (TraceGens.add_block c acts).
+
+Definition dexter_state env := get_contract_state Dexter.State env dexter_caddr.
+Definition token_state env := get_contract_state EIP20Token.State env token_caddr.
+
+Module TestInfo <: DexterTestsInfo.
+  Definition token_caddr := token_caddr.
+  Definition dexter_contract_addr := dexter_caddr.
+  Definition test_accounts := [person_1].
+End TestInfo.
+Module MG := DexterGens.DexterGens TestInfo. Import MG.
+
+(* Sample (gDexterAction chain1). *)
+
+(* Sample ((liftM (fun a => add_block_with_acts chain1 [a]) (gDexterAction chain1))). *)
+(* Sample (gDexterChain 2 chain1 1). *)
+
+Definition person_1_initial_balance : Amount := env_account_balances chain person_1.
+
+Definition dexter_liquidity chain : Amount := env_account_balances chain dexter_caddr.
+
+Definition account_tokens (env : Environment) (account : Address) : N :=
+  with_default 0%N (
+    do token_state <- token_state env ;
+    FMap.find account token_state.(EIP20Token.balances)
+    ).
+
+Definition dexter_token_pool (env : Environment) : N :=
+  with_default 0%N (
+    do s <- dexter_state env ;
+    Some s.(token_pool)
+    ).
+
+Open Scope Z_scope.
+Coercion Z.of_N : N >-> Z.
+
+(* Asserts that exchanges are priced correctly *)
+Definition tokens_to_asset_correct_P_opt (old_env new_env : Environment) : option Checker :=
+  do state_dexter <- dexter_state new_env;
+  let person_1_balance := env_account_balances new_env person_1 in
+  let dexter_balance := env_account_balances new_env dexter_caddr in
+  let dexter_initial_balance := env_account_balances old_env dexter_caddr in
+  let dexter_initial_token_reserve := account_tokens old_env dexter_caddr in
+  let dexter_current_token_reserve := account_tokens new_env dexter_caddr in
+  (* We assume only the given account has made exchanges in this time period.
+     This assumption holds for these tests. *)
+  let tokens_received := dexter_current_token_reserve - dexter_initial_token_reserve in
+  (* Calculate token exchange price if only a single exchange was made *)
+  let expected_currency_sold := getInputPrice tokens_received dexter_initial_token_reserve dexter_initial_balance in
+  let expected_dexter_balance := dexter_initial_balance - expected_currency_sold in
+  Some (
+    whenFail (
+      "dexter balance was " ++ show dexter_balance ++
+      " while it was expected to be at least " ++ show expected_dexter_balance ++ nl ++
+      "person_1 balance: " ++ show person_1_balance ++ nl ++
+      "person_1 tokens: " ++ show (account_tokens new_env person_1) ++ nl ++
+      "dexter balance: " ++ show dexter_balance ++ nl ++
+      "dexter tokens: " ++ show dexter_current_token_reserve ++ nl ++
+      "history: " ++ show (state_dexter.(price_history))
+    )
+    (checker (expected_dexter_balance <=? dexter_balance))
+  ).
+
+Definition tokens_to_asset_correct_P old_env env :=
+  match tokens_to_asset_correct_P_opt old_env env with
+  | Some p => p
+  | None => checker true
+  end.
+
+Definition tokens_to_asset_correct :=
+  forAllChainStatePairs 1 chain (gDexterChain 2) tokens_to_asset_correct_P.
+
+(* We first test the Dexter contract with breadth-first execution model *)
+(* QuickChick (tokens_to_asset_correct). *)
+(* +++ Passed 10000 tests (0 discards) *)
+(* We see that the property holds with breadt-first execution model *)
+
+(* However, the Dexter contract was designed for Tezos which used
+   breadth-first execution model.
+   Thus we next test the property with that model *)
+(* Extract Constant DepthFirst => "false".
+QuickChick (tokens_to_asset_correct). *)
+(*
+Chain{|
+Block 1 [
+Action{act_from: 10%256, act_body: (act_deploy 0, DexterSetup{token_caddr_: 10%256, token_pool_: 100})};
+Action{act_from: 10%256, act_body: (act_deploy 30, DexterSetup{token_caddr_: 128%256, token_pool_: 60})};
+Action{act_from: 10%256, act_body: (act_call 128%256, 0, DexterSetup{token_caddr_: 11%256, token_pool_: 40})};
+Action{act_from: 10%256, act_body: (act_call 128%256, 0, DexterSetup{token_caddr_: 129%256, token_pool_: 60})};
+Action{act_from: 11%256, act_body: (act_call 128%256, 0, approve 129%256 100)}];
+Block 2 [
+Action{act_from: 11%256, act_body: (act_call 129%256, 0, token_to_asset exchange{exchange_owner: 11%256, tokens_sold: 20})};
+Action{act_from: 11%256, act_body: (act_call 129%256, 0, token_to_asset exchange{exchange_owner: 11%256, tokens_sold: 14})}];|}
+
+dexter balance was 19 while it was expected to be at least 20
+person_1 balance: 11
+person_1 tokens: 6
+dexter balance: 19
+dexter tokens: 94
+history: [7; 4]
+*** Failed after 23 tests and 2 shrinks. (0 discards)
+*)
+
+(* We can see that the property fails in breadth-first model when two trades are made
+   in the same block. Below we simulate what goes wrong in this example.
+   The starting configuration is
+   person_1 balance: 10
+   person_1 tokens: 40
+   dexter balance: 30
+   dexter tokens: 60
+*)
+(* Compute (env_account_balances chain person_1). *)
+(* = 10 : N *)
+(* Compute (account_tokens chain person_1). *)
+(* = 40 : N *)
+(* Compute (env_account_balances chain dexter_caddr). *)
+(* = 30 : N *)
+(* Compute (account_tokens chain dexter_caddr). *)
+(* = 60 : N *)
+
+(* If both trades were merged person_1 would get 10 tez for his 34 tokens *)
+(* Compute (getInputPrice 34 60 30). *)
+(* = 10 : Z *)
+
+(* However, this is not what happens, in total person_1 gains 7+4=11 tez from
+   trading 34 tokens (20 in the first trade, 14 in the second) *)
+(* In the first trade person_1 trades 20 tokens for 7 tez *)
+(* Compute (getInputPrice 20 60 30). *)
+(* = 7 : Z *)
+(* In the second trade we would expect person_1 to get 3 tez for his 14 tokens *)
+(* Compute (getInputPrice 14 80 23). *)
+(* = 3 : Z *)
+(* However, this is not the calculation that is being done.
+   Instead the contract computes the yield of the second trade as follows *)
+(* Compute (getInputPrice 14 80 30). *)
+(* = 4 : Z *)
+(* This is because in breadth first execution model both trades gets started before tokens and tez
+   from previous trades have been transferred. Thus trades uses wrong values.
+   Dexter manually tracks and decrements the number of tokens in the reserve because of this.
+   However, the contract doesn't manually track tez the same way, thus the tez amount used is wrong. *)
