examples/escrow/tests/EscrowTests.v
@@ -25,14 +25,13 @@ Section TestSetup.
     setup_buyer := buyer
   |}.
 
-  Definition deploy_escrow amount := create_deployment amount Escrow.contract escrow_setup.
   Definition escrow_contract_addr : Address := contract_base_addr.
   (* The initial blockchain with the escrow contract deployed, and with buyer balance = 10 *)
   Definition escrow_chain : ChainBuilder :=
     unpack_result (TraceGens.add_block empty_chain
     [
-      build_act seller seller (act_transfer buyer 10);
-      build_act seller seller (deploy_escrow 2)
+      build_transfer seller buyer 10;
+      build_deploy seller 2 Escrow.contract escrow_setup
     ]).
     
 End TestSetup.
